add

src/coupon_collector/EvolvedCouponCollector.lean
@@ -1,6 +1,17 @@
 --import Paperproof
+/-
+think tags: next, next step
 
+for all tags t, for all store, if inserting a key,for all the 
+equuivalence tags hold 
+
+next step: any modification to KVStore should not break the equivalence relation 
+-/
 -- each key is String type for now
+
+import Std.Data.HashMap
+open Std 
+
 structure Tag where
   lhs : String 
   rhs : String
@@ -12,79 +23,103 @@ structure KVStore where
 
 -- same request,apply_coupon_collector functions below: 
  inductive Request --exposed to user
- | Identity : String → Request
+ | Reflexivity : String → Request -- changed needed
  | Symmetry : Tag → Request
  | Transitivity: Tag → Tag → Request --a structure: multi-args
  
+ -- reflexitivity 
  def apply_coupon_collector : Request → Option Tag
- | Request.Identity x       => some ({lhs := x, rhs := x})
+ | Request.Reflexivity x       => some ({lhs := x, rhs := x})
  | Request.Symmetry t       => some ({lhs := t.rhs, rhs := t.lhs})
  | Request.Transitivity t₁ t₂ => if t₁.rhs == t₂.lhs then some {lhs := t₁.lhs, rhs := t₂.rhs} else none
  
-/-
-Two ways to get an equivalence tag: from Tag struct or from KVStore
-Enforcing how KVStore should be updated: only when it doesn't break equivalence tag
--/
--- equivalenceTag function to issue a tag: assuming the keys already exist in the store
-
--- bypassing coupon collector to get a tag
+-- bypassing coupon collector to get a tag: check lhs rhs == none 
 def issue_equivalence_tag (store : KVStore) (lhs rhs : String) : Option Tag :=
-  if store.mapping lhs == store.mapping rhs then
+  if store.mapping lhs == store.mapping rhs ∧ 
+  store.mapping lhs != none then
     some { lhs := lhs, rhs := rhs }
   else
     none
 
--- via coupon collector to get equivalence tag
-def Tag.EquivalenceInvariant (store : KVStore)(t : Tag) : Bool := 
-  store.mapping t.lhs == store.mapping t.rhs
-
-def request_equivalence_tag (store : KVStore) (r : Request) : Option Tag :=
-  match apply_coupon_collector r with
-  | some t => if Tag.EquivalenceInvariant store t then some t else none
-  | none => none
+-- we don't want to insert a new key with same name as existing key but points to a diff value
+def KVStore.insert (store : KVStore) (key : String) (val : Nat) : Option KVStore := 
+  match store.mapping key with 
+  -- if inserted key has no existing value, then we insert new kv pair
+  | none => some {mapping := λ k => 
+              if k == key then some val else store.mapping k }
+  -- if inserted kv pair exists in the store, return old store, 
+  -- else if the key of the new kv pair points to a conflicting value of an existing key
+  -- we also return old store
+  | some _ => store
 
 -- we don't want KVStore to delete a key if the key is still pointing to the value 
--- or inserting a new key with same name as existing key but points to a diff value
-def KVStore.insert (store : KVStore) (key : String) (val : Nat) : Bool := 
-  match store.mapping key with 
-  | none => true
-  | some existing_val => existing_val == val 
-
 -- return an updated store after deletion 
 def KVStore.delete (store : KVStore) (key : String) : Option KVStore := 
-  match store.mapping key with 
-  | none => none 
-  | some _ => 
-      some {
-        mapping := λ k => 
-          if k == key then none else store.mapping k 
-      }
+  some {mapping := λ k => 
+          if k == key then none else store.mapping k } 
 
--- some test cases of the functions above:  
-def test_store : KVStore := 
-  {mapping := λ key => 
-  if key = "a" then some 42
-  else if key = "b" then some 42 
-  else if key = "c" then some 5
-  else none}
-#eval issue_equivalence_tag test_store "a" "b"
-#eval request_equivalence_tag test_store (Request.Identity "a")
-#eval request_equivalence_tag test_store (Request.Symmetry {lhs := "a", rhs :="b"})
-#eval KVStore.insert test_store "d" 1
-#eval match KVStore.delete test_store "b" with
-  | some newStore => newStore.mapping "a"  -- should be none
-  | none => none
+-- implement KVStore by hashmap: 
+
+def insert (m : HashMap String Nat) (key : String) (val : Nat) : 
+Option (HashMap String Nat) :=
+  if m.contains key then none else some (m.insert key val)
+
+def delete (m : HashMap String Nat) (key : String) : 
+HashMap String Nat :=
+  m.erase key
+
+def all_tags_value_true (m : HashMap String Nat) (ts : List Tag) : 
+Bool :=
+  ts.all (λ t => m.get? t.lhs == m.get? t.rhs)
+
+-- tests for HashMap based KVStore: 
+def testStore: HashMap String Nat := HashMap.empty.insert "x" 1 
+#eval insert testStore "x" 2  -- should return `none`
+#eval insert testStore "y" 2  -- should return `some (map with "x" -> 1, "y" -> 2)`
+
+
 -- coupon collector trusts the authorship 
 -- store should be trusted: what is store responsible for? 
--- keys cann be inseted/deleted 
+-- keys can be inseted/deleted 
 
 def Request.toList : Request -> List Tag
-  | Request.Identity _ => []
+  | Request.Reflexivity _ => []
   | Request.Symmetry t => [t]
   | Request.Transitivity t₁ t₂ => [t₁, t₂]
 
 def all_tag_true (store : KVStore) (ts: List Tag) : Bool :=
   ts.all λ t => store.mapping t.lhs == store.mapping t.rhs -- runtime check 
+
+/-
+theorem: for all collection of tags ts, for all stores, for all storage operations, if all equivalence tags ts are true before, 
+they are still true afterwards 
+
+Note: we should break down this kvstore to prove for insertion/deletion separately; 
+otherwise, the proof will get very complicated and buggy
+-/
+
+/-
+∀ (m : KVStore) (ts : List Tag) (key : String) (val : Nat) (m' : KVStore)  ≡ 
+∀ (m : KVStore) ∀ (ts : List Tag) ∀ (key : String) ∀ (val : Nat) ∀ (m' : KVStore)
+Lean interprets: 
+ ∀ (x : A) (y : B) (z : C), P x y z the same way as 
+ (∀ x : A) → (∀ y : B) → (∀ z : C) → P x y z
+  ∀ is the syntatic sugar for dependent type binding
+reference: https://github.com/soonhokong/lean-tutorial/blob/master/04_Quantifiers_and_Equality.org
+
+ How do we interpret nested →: A → B →  C: if A then B then C
+ reference: https://www.imo.universite-paris-saclay.fr/~patrick.massot/mil/03_Logic.html 
+
+
+-/
+      
+theorem insertion_soundness_proof :
+  ∀ (m : KVStore) (ts : List Tag) (key : String) (val : Nat) (m' : KVStore),
+    all_tag_true m ts = true ∧ 
+    KVStore.insert m key val = some m' →
+    all_tag_true m' ts = true := by sorry 
+
+    
 
 
 theorem soundness_proof : 
@@ -93,7 +128,7 @@ theorem soundness_proof :
     all_tag_true store (Option.toList (apply_coupon_collector r)) := by -- apply_coupon_collector r.toList
   intros r store h 
   cases r with 
-    | Identity x => 
+    | Reflexivity x => 
       simp [Request.toList, Option.toList, all_tag_true, apply_coupon_collector]
       
     -- h : (store.mapping t.lhs == store.mapping t.rhs) = true
@@ -130,10 +165,13 @@ theorem soundness_proof :
       
           case true =>
             simp [apply_coupon_collector, cond, Option.toList, all_tag_true]
+            -- ∀ x ∈ [a], p x ↔ p a useful for store mapping 
             apply List.forall_mem_singleton.2
             simp at h₁ h₂
             have cond_eq : t₁.rhs = t₂.lhs := of_decide_eq_true cond
             have map_eq : store.mapping t₁.rhs = store.mapping t₂.lhs :=
+                -- CongrArg: if we have f a = f b as a goal and we know 
+                --a = b, we can use a =b to replace the goal 
                 congrArg store.mapping cond_eq
             have h₂' : store.mapping t₁.rhs = store.mapping t₂.rhs :=
                map_eq.trans h₂
@@ -142,4 +180,18 @@ theorem soundness_proof :
       
          
      
-  
+-- some test cases of the KVStore functions above:  
+def test_store : KVStore := 
+  {mapping := λ key => 
+  if key = "a" then some 42
+  else if key = "b" then some 42 
+  else if key = "c" then some 5
+  else if key = "e" then none
+  else none}
+#eval issue_equivalence_tag test_store "a" "b"
+#eval match KVStore.insert test_store "d" 1 with
+  | some newStore => newStore.mapping "d"  -- should be 1
+  | none => none
+#eval match KVStore.delete test_store "b" with
+  | some newStore => newStore.mapping "b"  -- should be none
+  | none => none
